Counter-example for the inductive definition

CTree.v
@@ -1,70 +1,33 @@
-From RelationAlgebra Require Import
-     kat
-     kat_tac
-     prop
-     rel
-     srel
-     comparisons
-     rewriting
-     normalisation
-     monoid.
 From CTree Require Import CTree Eq.
-From OptSim Require Import OptSim.
+From OptSim Require Import Utils LTS OptSim.
+
+Import CoindNotations.
+
 
 Variant olabel {E} :=
 | oobs {X} : E X -> X -> olabel
 | oval {X} : X -> olabel.
 
-Definition clabel {E} (l : @OptSim.label (@olabel E)) :=
+Definition clabel {E} (l : @LTS.label (@olabel E)) :=
   match l with
   | tau => τ
-  | OptSim.obs (oobs e x) => Trans.obs e x
-  | OptSim.obs (oval v) => val v
+  | LTS.obs (oobs e x) => Trans.obs e x
+  | LTS.obs (oval v) => val v
   end.
 
 Program Definition lts {E B X} : LTS :=
 {|
   Observable := @olabel E;
   St := @SS E B X;
-  OptSim.trans := fun l => {| hrel_of := Trans.trans (clabel l) |};
+  LTS.trans := fun l => {| hrel_of := Trans.trans (clabel l) |};
   epsilon := {| hrel_of := fun _ _ => False |};
   Robs := eq;
   ub_state := fun _ => False
 |}.
 
-Import CTreeNotations.
-CoFixpoint t : ctree void1 B2 bool := brS2 t (branchS branch2).
-CoFixpoint u : ctree void1 B2 bool := r <- branchS branch2;; brS2 u (Ret r).
-
-Lemma unfold_t : t = brS2 t (branchS branch2). Admitted.
-Lemma unfold_u : u = r <- branchS branch2;; brS2 u (Ret r). Admitted.
-
-Goal sim lts SimOpt.div SimOpt.nolock SimOpt.expand t u.
+#[export] Instance Chain_simF_equ E B X freeze lock delay b : forall (R : Chain (simF (lts := lts) freeze lock delay)),
+  Proper (@equ E B X X eq ==> equ eq ==> impl) (`R b).
 Proof.
-  red. coinduction R CH.
-  rewrite unfold_t, unfold_u.
-  cbn. constructor. repeat split; intros.
-  1, 3: admit.
-  apply tau_div. reflexivity.
-  cbn in H. apply trans_brS_inv in H as (? & ? & _).
-  rewrite H. destruct x.
-Abort.
-
-Goal gfp (divsimF lts SimOpt.nolock) t u.
-Proof.
-  coinduction R CH.
-  repeat split; intros.
-  1, 4: admit.
-  - (*cbn -[str] in H. eapply srel_str_ind_l' with (i := trans τ) (P := fun t s' => exists t' : St lts, (OptSim.trans lts tau)^* u t' /\ ` R s' t').
-    4: apply H.
-    + cbn. intros. subs. admit.
-    + intros. *)
-   assert (s' = t \/ s' = branchS branch2 \/ s' = Ret true \/ s' = Ret false) by admit.
-   destruct H0 as [|[|[|]]]; subst.
-   + exists u. split; auto. rewrite <- str_refl. reflexivity.
-   + exists u. split; auto. now rewrite <- str_refl. admit.
-   + exists (Ret true). split. rewrite str_unfold_l. right. rewrite <- str_ext. cbn. rewrite unfold_u. red. eexists. unfold branchS. rewrite bind_br. eapply trans_br. 2: reflexivity.
-     rewrite bind_step. apply trans_step. rewrite bind_ret_l. apply trans_brS22. admit.
-   + admit.
- - admit.
-Admitted.
+  intros. cbn. intros.
+  eapply (Chain_simF_eq'' (lts := lts)); eauto.
+Qed.
