IndSim.v
@@ -11,17 +11,20 @@ From RelationAlgebra Require Import
 From Coinduction Require Import all.
 From OptSim Require Import Utils LTS OptSim.
 
+Import CoindNotations.
+
+
 Section WithLTS.
 
 Context {lts : LTS}.
 Context (freeze : SimOpt.freeze_opt) (lock : SimOpt.lock_opt) (delay : SimOpt.delay_opt).
-Let Observable := lts.(Observable).
-Let St := lts.(St).
-Let trans := lts.(trans).
-Let epsilon := lts.(epsilon).
-Let Robs := lts.(Robs).
-Let ub_state := lts.(ub_state).
-Let label := @label Observable.
+Notation Observable := lts.(Observable).
+Notation St := lts.(St).
+Notation trans := lts.(trans).
+Notation epsilon := lts.(epsilon).
+Notation Robs := lts.(Robs).
+Notation ub_state := lts.(ub_state).
+Notation label := (@label Observable).
 
   (* TODO try to just use TauAnswer with Rind as Rdiv *)
   Variant TauIndAnswer (R Rind : relation St) s' t : Prop :=
@@ -37,9 +40,9 @@ Let label := @label Observable.
       ObsAnswer delay R s' t o
     ) /\
     (forall s', trans tau s s' ->
-      TauIndAnswer R Rind s' t
+      TauAnswer freeze delay R Rind s' t
     ) /\
-    (lock = SimOpt.nolock \/ (is_stuck s -> is_stuck t)).
+    (lock = SimOpt.nolock \/ (is_stuck s -> can_be_stuck delay t)).
 
   Section NoElim.
   #[local] Unset Elimination Schemes.
@@ -68,8 +71,45 @@ Proof.
   repeat split; intros.
   - apply H0 in H1 as []; esim.
   - apply H0 in H1 as []; esim.
-    destruct SIM. esim.
+    destruct DIV. esim.
   - apply H0.
+Qed.
+
+Program Definition isimF : mon (St -> St -> Prop) :=
+{| body R s t := simInd R s t |}.
+Next Obligation.
+  eapply simInd_mon. 2: apply H0.
+  cbn. apply H.
+Qed.
+
+#[export] Instance Chain_isimF_eq : forall (R : Chain isimF),
+  Proper (Eq St ==> Eq St ==> impl) `R.
+Proof.
+  intro. apply tower. {
+    intros ? INC ?????????. eapply INC; eauto.
+  }
+  intros. cbn. intros; subst.
+  revert y y0 H0 H1. induction H2. intros.
+  repeat split; intros.
+  - rewrite <- H2. rewrite <- H1 in H3. now apply H0 in H3.
+  - rewrite <- H1 in H3. apply H0 in H3 as []; rewrite ?H2 in *; esim.
+    apply tau_div; auto. now eapply DIV.
+  - rewrite <- H1, <- H2. apply H0.
+Qed.
+
+Definition isim := gfp isimF.
+
+Theorem sim_indsim : forall s t ,
+  isim s t ->
+  sim freeze lock delay true s t.
+Proof.
+  red. coinduction R CH. intros.
+  apply (gfp_fp isimF) in H. induction H.
+  apply simF_equiv. repeat split; intros.
+  - apply H in H0 as []; esim.
+  - apply H in H0 as []; esim.
+    apply tau_div; auto. apply simF_f_t. now rewrite H0. apply DIV.
+  - apply H.
 Qed.
 
 End WithLTS.
