IndSimCounterExample.v
@@ -1,0 +1,97 @@
+From RelationAlgebra Require Import
+     kat
+     kat_tac
+     prop
+     rel
+     srel
+     comparisons
+     rewriting
+     normalisation
+     monoid.
+From CTree Require Import CTree Eq.
+From OptSim Require Import Utils LTS Divergence OptSim IndSim CTree.
+
+Import CoindNotations.
+Import CTreeNotations.
+
+CoFixpoint t : ctree void1 (B2 +' B3) bool := brS3 t (Ret true) (Ret false).
+CoFixpoint u' r : ctree void1 (B2 +' B3) bool := brS2 (u' r) (Ret r).
+Definition u : ctree void1 (B2 +' B3) bool := brS branch2 u'.
+
+Lemma unfold_t : t = brS3 t (Ret true) (Ret false). Admitted.
+Lemma unfold_u' r : u' r = brS2 (u' r) (Ret r). Admitted.
+
+Lemma negb_ret_u' : forall x, isim (lts := lts) SimOpt.freeze_div SimOpt.nolock SimOpt.delay (Ret (negb x)) (u' x) -> False.
+Proof.
+  intros. apply (gfp_fp (isimF _ _ _)) in H.
+  remember (Ret (negb x)). remember (u' x). induction H. subst. rewrite unfold_u' in H.
+  destruct H as (? & _ & _). specialize (H (oval (negb x)) Stuck).
+  lapply H. 2: { cbn. apply trans_ret. }
+  clear H. intro. destruct H.
+  - apply trans_brS_inv in TR as (? & ? & ?).
+    cbn in OBS. subst. discriminate.
+  - admit.
+Admitted.
+
+Lemma t_u' : forall x, isim (lts := lts) SimOpt.freeze_div SimOpt.nolock SimOpt.delay t (u' x) -> False.
+Proof.
+  intros. apply (gfp_fp (isimF _ _ _)) in H.
+  remember t. remember (u' x). destruct H. subst. rewrite unfold_t, unfold_u' in H.
+  destruct H as (_ & ? & _). specialize (H (Ret (negb x))).
+  lapply H. 2: { cbn. eapply trans_br with (x := match x with true => t33 | false => t32 end). 2: reflexivity. destruct x; etrans. }
+  clear H. intro. destruct H.
+  - apply trans_brS_inv in TR as ([] & ? & _); subs.
+    + now eapply negb_ret_u' in SIM.
+    + admit.
+  - discriminate.
+  - rewrite <- unfold_u' in SIM. now apply negb_ret_u' in SIM.
+  - admit.
+Admitted.
+
+Goal isim (lts := lts) SimOpt.freeze_div SimOpt.nolock SimOpt.delay t u -> False.
+Proof.
+  intros. apply (gfp_fp (isimF _ _ _)) in H.
+  remember t. remember u. induction H. subst. rewrite unfold_t in H. unfold u in H.
+  destruct H as (_ & ? & _). specialize (H t).
+  lapply H. 2: { cbn. apply trans_brS31. }
+  clear H. intro. destruct H.
+  - apply trans_br_inv in TR as [].
+    apply trans_step_inv in H as [? _]. rewrite H in SIM.
+    clear t' H.
+    now apply t_u' in SIM.
+  - discriminate.
+  - destruct DIV. apply H1. apply unfold_t. reflexivity.
+  - admit.
+Admitted.
+
+Lemma u_div : diverges (lts := lts) u.
+Proof.
+  red. coinduction R CH.
+  exists (u' true). split.
+  - unfold u. apply trans_brS.
+  - accumulate R'. exists (u' true).
+    split; auto. rewrite unfold_u' at 1.
+    apply trans_brS21.
+Qed.
+
+Goal sim (lts := lts) SimOpt.freeze_div SimOpt.nolock SimOpt.delay true t u.
+Proof.
+  red. coinduction R CH.
+  rewrite unfold_t. unfold u.
+  cbn. constructor. repeat split; intros.
+  1, 3: admit.
+  cbn in H. apply trans_brS_inv in H as (? & ? & _).
+  subs. destruct x.
+  - apply tau_div; auto.
+    apply (gfp_chain R).
+    apply diverges_divpres.
+    apply u_div.
+  - eapply tau_delay; auto.
+    2: apply (upto_refl (lts := lts)); auto.
+    rewrite itr_str_l.
+    unfold branchS.
+    esplit. eapply trans_br with (x := true). 2: reflexivity. apply trans_step.
+    rewrite unfold_u'. rewrite <- str_ext. eapply trans_br with (x := false).
+    2: reflexivity. apply trans_step.
+  - admit.
+Admitted.
